DAG stuff

DAG.dfy
@@ -1,32 +1,106 @@
-// RUN: /compile:0
+// RUN: /compile:0 /rlimit:1000000
+
+datatype Graph<A> = Graph(nodes: set<A>, edges: set<(A,A)>)
+
+predicate ValidGraph<A>(g: Graph<A>)
+{
+    var Graph(nodes, edges) := g;
+    forall u, v | (u, v) in edges :: u in nodes && v in nodes
+}
+
+type Path<A> = seq<A>
+
+predicate ValidPath<A>(g: Graph<A>, p: Path<A>)
+{
+    && |p| > 0
+    && p[0] in g.nodes
+    && forall i | 0 <= i < |p|-1 :: (p[i], p[i+1]) in g.edges
+}
+
+function last<A>(s: seq<A>): A
+    requires |s| > 0
+{
+    s[|s| - 1]
+}
+
+predicate ValidDAG<A>(g: Graph<A>)
+{
+    && ValidGraph(g)
+    && forall p | ValidPath(g, p) :: |p| > 1 ==> p[0] != last(p)
+}
+
+predicate DiamondNode(i: int)
+{
+    0 <= i < 4
+}
+
+function DiamondDAG(): Graph<int>
+{
+    Graph(set i {:nowarn} | 0 <= i < 4,
+          set i, j |
+              && 0 <= i < 4
+              && 0 <= j < 4
+              && (|| (i == 0 && j == 1)
+                 || (i == 0 && j == 2)
+                 || (i == 1 && j == 3)
+                 || (i == 2 && j == 3))
+              :: (i, j))
+}
+
+lemma lemma_DiamondDAGValid()
+    ensures ValidDAG(DiamondDAG())
+{
+    var g := DiamondDAG();
+    forall p | ValidPath(g, p) && |p| > 1
+        ensures p[0] != last(p)
+    {
+        assert (p[0], p[1]) in g.edges;
+        assert |p| > 2 ==> (p[1], p[2]) in g.edges;
+        assert |p| > 3 ==> (p[2], p[3]) in g.edges;
+    }
+}
 
 class Node {
     var children: set<Node>
     ghost var repr: set<object>
-    
-    predicate Valid()
+
+    predicate LocallyValid()
         reads this, repr
     {
         && this in repr
         && null !in repr
-        && forall x | x in children :: 
+        && forall x | x in children ::
             && x in repr
             && x.repr <= repr
-            && this !in x.repr
-            && x.Valid()
     }
 
-    predicate Reachable(c: Node)
+    predicate DAGValid()
         reads this, repr
-        requires Valid()
+    {
+        && LocallyValid()
+        && forall x | x in children ::
+            && this !in x.repr
+            && x.DAGValid()
+    }
+
+    predicate LocallyRespectsGraph(g: Graph<Node>)
+        reads this
+    {
+        && this in g.nodes
+        && children == set p | p in g.edges && p.0 == this :: p.1
+    }
+
+    predicate PathTo(c: Node)
+        reads this, repr
+        requires DAGValid()
     {
         || c == this
-        || exists x | x in children :: x.Reachable(c)
+        || exists x | x in children :: x.PathTo(c)
     }
 
     constructor(children: set<Node>) 
-        requires forall c | c in children :: c != null && c.Valid()
-        ensures Valid()
+        requires forall c | c in children :: c != null && c.DAGValid()
+        ensures DAGValid()
     {
         this.children := children;
         repr := {};
@@ -47,38 +121,97 @@ class Node {
     }
 }
 
+predicate GraphGloballyReflected(g: Graph<Node>)
+    reads g.nodes
+{
+    && null !in g.nodes
+    && forall n | n in g.nodes :: n.LocallyRespectsGraph(g)
+}
+
+
+lemma lemma_PathToPathHelper(g: Graph<Node>, x: Node, y: Node) returns (p: Path<Node>)
+    requires ValidGraph(g) && GraphGloballyReflected(g)
+    requires x in g.nodes && x.DAGValid()
+    requires x.PathTo(y)
+    ensures ValidPath(g, p) && p[0] == x && last(p) == y
+    decreases x.repr
+{
+    if x == y {
+        p := [x];
+    } else {
+        var c :| c in x.children && c.PathTo(y);
+        var q := lemma_PathToPathHelper(g, c, y);
+        p := [x] + q;
+    }
+}
+
+lemma lemma_PathToPath(g: Graph<Node>)
+    requires ValidGraph(g) && GraphGloballyReflected(g)
+    requires forall x | x in g.nodes :: x.DAGValid()
+    ensures forall x, y | x in g.nodes && y in g.nodes && x.PathTo(y) ::
+        exists p :: ValidPath(g, p) && p[0] == x && last(p) == y
+{
+    forall x, y | x in g.nodes && y in g.nodes && x.PathTo(y)
+        ensures exists p :: ValidPath(g, p) && |p| > 0 && p[0] == x && last(p) == y
+    {
+        var p := lemma_PathToPathHelper(g, x, y);
+    }
+}
+
+lemma lemma_PathPathToHelper(g: Graph<Node>, p: Path<Node>)
+    requires ValidGraph(g) && GraphGloballyReflected(g)
+    requires ValidPath(g, p)
+    requires forall x | x in g.nodes :: x.DAGValid()
+    ensures p[0].PathTo(last(p))
+{
+    if |p| != 1 {
+        lemma_PathPathToHelper(g, p[1..]);
+    }
+}
+
+
 class TopoSort {
     var result: seq<Node>
 
     method Visit(n: Node)
-        requires n != null && n.Valid() 
+        requires n != null && n.DAGValid()
         requires this !in n.repr 
         requires forall x | x in result :: 
             && x != null 
             && this !in x.repr
-            && x.Valid()
-            && (forall y | x.Reachable(y) :: y in result)
+            && x.DAGValid()
+            && (forall y | x.PathTo(y) :: y in result)
+        /*requires forall i, j | 0 <= i < j < |result| ::
+            result[j] in result && !result[j].PathTo(result[i])*/
         decreases n.repr
         modifies this
         ensures forall x | x in old(result) :: x in result
-        ensures forall x | n.Reachable(x) :: x in result
+        ensures forall x | n.PathTo(x) :: x in result
         ensures forall x | x in result :: 
             && x != null 
             && this !in x.repr
-            && x.Valid()
-            && (forall y | x.Reachable(y) :: y in result)
+            && x.DAGValid()
+            && (forall y | x.PathTo(y) :: y in result)
+        /*ensures forall i, j | 0 <= i < j < |result| ::
+            result[j] in result && !result[j].PathTo(result[i])
+        ensures forall x | x in result :: x in old(result) || n.PathTo(x)*/
     {
         if n in result { return; }
+        assert n !in result;
         var S := n.children;
         while S != {}
             decreases S
+//            invariant n !in result
             invariant forall x | x in old(result) :: x in result
             invariant forall x | x in n.children :: x in S || x in result
             invariant forall x | x in result :: 
                 && x != null 
                 && this !in x.repr
-                && x.Valid()
-                && (forall y | x.Reachable(y) :: y in result)
+                && x.DAGValid()
+                && (forall y | x.PathTo(y) :: y in result)
+            /*invariant forall i, j | 0 <= i < j < |result| ::
+                result[j] in result && !result[j].PathTo(result[i])
+            invariant forall x | x in result :: x in old(result) || n.PathTo(x) */
         {
             var x :| x in S;
             Visit(x);
@@ -88,28 +221,39 @@ class TopoSort {
     }
 }
 
-method TopoSort(nodes: set<Node>) returns (s: seq<Node>)
-    requires forall n | n in nodes :: n != null && n.Valid()
-    ensures forall n | n in nodes :: forall x | n.Reachable(x) :: x in s
+lemma lemma_IndexInSeq<A>(i: int, s: seq<A>)
+    requires 0 <= i < |s|
+    ensures s[i] in s
+{}
+
+
+method TopoSort(roots: set<Node>) returns (s: seq<Node>)
+    requires forall n | n in roots :: n != null && n.DAGValid()
+    ensures forall n | n in roots :: forall x | n.PathTo(x) :: x in s
+    ensures forall n | n in s :: n != null && n.DAGValid()
+//    ensures forall i, j | 0 <= i < j < |s| :: s[j] in s && !s[j].PathTo(s[i])
 {
     var state := new TopoSort;
     state.result := [];
     
-    var S := nodes;
+    var S := roots;
     while S != {}
         decreases S
-        invariant forall n' | n' in nodes :: state !in n'.repr;
-        invariant forall n: Node | n in nodes && n !in S :: forall x | n.Reachable(x) :: x in state.result
+        invariant forall n' | n' in roots :: state !in n'.repr;
+        invariant forall n: Node | n in roots && n !in S :: forall x | n.PathTo(x) :: x in state.result
         invariant forall x | x in state.result :: 
             && x != null 
             && state !in x.repr
-            && x.Valid()
-            && (forall y | x.Reachable(y) :: y in state.result)
+            && x.DAGValid()
+            && (forall y | x.PathTo(y) :: y in state.result)
+/*        invariant forall i, j | 0 <= i < j < |state.result| ::
+            state.result[j] in state.result &&
+            !state.result[j].PathTo(state.result[i])*/
     {
         var n :| n in S;
         state.Visit(n);
         S := S - {n};
     }
 
-    return state.result;
+    s := state.result;
 }
